Added fifo, renamed

formalization/Push_Relabel_Maxflow/evaluation/rtof-SML/Rtof_Export.sml
@@ -249,15 +249,16 @@ end;
 
 
 
-    fun array_blit src si dst di len = 
+    fun array_blit src si dst di len = (
+      src=dst andalso raise Fail ("array_blit: Same arrays");
       ArraySlice.copy {
-        di=di,
-        src = ArraySlice.slice (src,si,SOME len),
-        dst=dst}
+        di = IntInf.toInt di,
+        src = ArraySlice.slice (src,IntInf.toInt si,SOME (IntInf.toInt len)),
+        dst = dst})
 
-    fun array_nth_oo v a i () = Array.sub(a,i) handle Subscript => v
+    fun array_nth_oo v a i () = Array.sub(a,IntInf.toInt i) handle Subscript => v | Overflow => v
     fun array_upd_oo f i x a () = 
-      (Array.update(a,i,x); a) handle Subscript => f ()
+      (Array.update(a,IntInf.toInt i,x); a) handle Subscript => f () | Overflow => f ()
 
     
 
@@ -374,12 +375,6 @@ structure Rtof : sig
   val prepareNet :
     (nat * (nat * int)) list ->
       nat -> nat -> ((nat * nat -> int) * ((nat -> nat list) * nat)) option
-  val relabel_to_front_impl :
-    (nat * nat -> int) ->
-      nat -> nat -> nat -> nat -> (nat list) array -> (unit -> (int array))
-  val relabel_to_front_impl_tab_am :
-    (nat * nat -> int) ->
-      nat -> nat -> nat -> (nat -> nat list) -> (unit -> (int array))
   val relabel_to_front :
     (nat * (nat * int)) list ->
       nat ->
@@ -1814,22 +1809,26 @@ datatype ('a, 'b) pre_network_ext =
 datatype ('a, 'b, 'c) simple_state_nos_impl_ext =
   Simple_state_nos_impl_ext of 'a * 'b * 'c;
 
-fun len A_ a = (fn () => let
-                           val i = (fn () => Array.length a) ();
-                         in
-                           nat_of_integer i
-                         end);
+fun len A_ a =
+  (fn () => let
+              val i = (fn () => IntInf.fromInt (Array.length a)) ();
+            in
+              nat_of_integer i
+            end);
 
-fun new A_ = (fn a => fn b => (fn () => Array.array (a, b))) o integer_of_nat;
+fun new A_ =
+  (fn a => fn b => (fn () => Array.array (IntInf.toInt a, b))) o integer_of_nat;
 
-fun nth A_ a n = (fn () => Array.sub (a, integer_of_nat n));
+fun nth A_ a n = (fn () => Array.sub (a, IntInf.toInt (integer_of_nat n)));
 
 fun upd A_ i x a =
-  (fn () => let
-              val _ = (fn () => Array.update (a, integer_of_nat i, x)) ();
-            in
-              a
-            end);
+  (fn () =>
+    let
+      val _ =
+        (fn () => Array.update (a, IntInf.toInt (integer_of_nat i), x)) ();
+    in
+      a
+    end);
 
 fun fold f (x :: xs) s = fold f xs (f x s)
   | fold f [] s = s;
@@ -1843,7 +1842,8 @@ fun map f [] = []
 fun image f (Set xs) = Set (map f xs);
 
 fun make A_ n f =
-  (fn () => Array.tabulate (integer_of_nat n, f o nat_of_integer));
+  (fn () => Array.tabulate (IntInf.toInt (integer_of_nat n),
+    (f o nat_of_integer) o IntInf.fromInt));
 
 fun map_of A_ ((l, v) :: ps) k = (if eq A_ l k then SOME v else map_of A_ ps k)
   | map_of A_ [] k = NONE;
