formalization/Push_Relabel_Maxflow/evaluation/printall.sh
@@ -2,12 +2,12 @@
 
 tests=`cat tests`
 platforms_fofu=`cat fofu-platforms`
-platforms_rtof=`cat rtof-platforms`
+platforms_fifo=`cat fifo-platforms`
 
 tabs -9
 echo -ne "Name \t& "
 for p in $platforms_fofu; do echo -ne "f-$p\t& "; done
-for p in $platforms_rtof; do echo -ne "p-$p\t& "; done
+for p in $platforms_fifo; do echo -ne "p-$p\t& "; done
 
 echo ""
 
@@ -19,8 +19,8 @@ for t in $tests; do
     echo -ne "$time\t& "
   done
   
-  for p in $platforms_rtof; do
-    log="rtof-$p/$t.$p.log"
+  for p in $platforms_fifo; do
+    log="fifo-$p/$t.$p.log"
     time=`grep "@@@time:" $log | sed -re 's/.*@@@time: //g;s/ms//g'`
     echo -ne "$time\t& "
   done
